an update

SimpleCurrencyExchange/SimpleCurrencyExchange-Cmover.bpl
@@ -2,18 +2,17 @@
 // A trade can be accessed by only the process that added it
 
 type Uid;
-type Tid;
 
-function {:builtin "MapConst"} MapConstBool(bool) : [Tid]bool;
-function {:inline} {:linear "tid"} TidCollector(x: Tid) : [Tid]bool
+function {:builtin "MapConst"} MapConstBool(bool) : [Uid]bool;
+function {:inline} {:linear "uid"} TidCollector(x: Uid) : [Uid]bool
 {
   MapConstBool(false)[x := true]
 }
 
 
 // shared variables
-var {:layer 0,2} tradeContents: [Tid][int]int;
-var {:layer 0,2} tradeUser: [Tid]Uid;
+var {:layer 0,2} tradeContents: [int][int]int;
+var {:layer 0,2} tradeUser: [Uid]int;
 
 // constants 
 const unique cstCurFr:int;
@@ -24,11 +23,24 @@ const unique cstRate   :int;
 const unique cstTiPl   :int;
 const unique cstoCount :int;
 
+const unique Owner : Uid;
 
-procedure {:right}{:layer 2}  saveTrade({:linear "tid"} tid:Tid, uid:Uid, curFr:int, curTo:int, sAmt:int, bAmt:int, rate:int, tiPl:int, oCount:int)
+
+procedure {:atomic}{:layer 2}  saveTradeR({:linear "uid"} uid:Uid) returns (tid:int)
 modifies tradeUser, tradeContents;
 {  
-   tradeUser[tid] := uid;
+   assume(uid != Owner);
+   tid = tradeUser[uid] + 1;
+}
+procedure{:yields}{:layer 1} {:refines "saveTradeR"} SaveTradeR({:linear "tid"} uid:Uid) returns (tid:int);
+
+
+procedure {:atomic}{:layer 2}  saveTradeW({:linear "uid"} uid:Uid, curFr:int, curTo:int, sAmt:int, bAmt:int, rate:int, tiPl:int, oCount:int)
+modifies tradeUser, tradeContents;
+{  
+   assume(uid != Owner);
+   var tid : int;
+   tradeUser[uid] := tid;
    
    tradeContents[tid][cstCurFr] := curFr;
    tradeContents[tid][cstCurTo] := curTo;
@@ -39,25 +51,28 @@ modifies tradeUser, tradeContents;
    tradeContents[tid][cstoCount] := oCount;
    
 }
-procedure{:yields}{:layer 1} {:refines "saveTrade"} SaveTrade({:linear "tid"} tid:Tid, uid:Uid, curFr:int, curTo:int, sAmt:int, bAmt:int, rate:int, tiPl:int, oCount:int);
+procedure{:yields}{:layer 1} {:refines "saveTradeW"} SaveTradeW({:linear "uid"} uid:Uid, curFr:int, curTo:int, sAmt:int, bAmt:int, rate:int, tiPl:int, oCount:int);
 
 
-procedure {:right}{:layer 2} viewTrade({:linear "tid"} tid:Tid) returns (cpTradeContent:[int]int)
+procedure {:atomic}{:layer 2} viewTrade({:linear "tid"} uid:Uid, tid: int) returns (cpTradeContent:[int]int)
 {
+  assume(uid == Owner);
   cpTradeContent := tradeContents[tid];
 }
-procedure {:yields}{:layer 1} {:refines "viewTrade"} ViewTrade({:linear "tid"} tid:Tid) returns (cpTradeContent:[int]int);
+procedure {:yields}{:layer 1} {:refines "viewTrade"} ViewTrade({:linear "tid"} uid:Uid, tid: int) returns (cpTradeContent:[int]int);
 
 
-procedure {:right}{:layer 2} viewTradeUser({:linear "tid"} tid:Tid) returns (cpTradeUser:Uid)
+procedure {:atomic}{:layer 2} viewTradeUser({:linear "tid"} uid:Uid, tid: int) returns (cpTradeUser:Uid)
 {
+  assume(uid == Owner);
   cpTradeUser := tradeUser[tid]; 
 }
-procedure {:yields}{:layer 1} {:refines "viewTradeUser"} ViewTradeUser({:linear "tid"} tid:Tid) returns (cpTradeUser:Uid);
+procedure {:yields}{:layer 1} {:refines "viewTradeUser"} ViewTradeUser({:linear "tid"} uid:Uid, tid: int) returns (cpTradeUser:Uid);
 
 
-procedure {:right}{:layer 2} getTradeTimeStamp({:linear "tid"} tid:Tid) returns (timeTrade:int)
+procedure {:atomic}{:layer 2} getTradeTimeStamp({:linear "tid"} uid:Uid, tid: int) returns (timeTrade:int)
 {
+  assume(uid == Owner);
   timeTrade:=tradeContents[tid][cstTiPl]; 
 }
-procedure {:yields}{:layer 1} {:refines "getTradeTimeStamp"} GetTradeTimeStamp({:linear "tid"} tid:Tid) returns (timeTrade:int);
+procedure {:yields}{:layer 1} {:refines "getTradeTimeStamp"} GetTradeTimeStamp({:linear "tid"} uid:Uid, tid: int) returns (timeTrade:int);
