Betting/Betting-Original.bpl
@@ -1,0 +1,46 @@
+// Betting Module
+// Transaction settleBet can be called only by one process
+
+type Pid;
+type Bid;
+
+function {:builtin "MapConst"} MapConstBoolPid(bool) : [Pid]bool;
+function {:inline} {:linear "Pid"} PidCollector(x: Pid) : [Pid]bool
+{
+  MapConstBoolPid(false)[x := true]
+}
+
+function {:builtin "MapConst"} MapConstBoolBid(bool) : [Bid]bool;
+function {:inline} {:linear "Bid"} BidCollector(x: Bid) : [Bid]bool
+{
+  MapConstBoolBid(false)[x := true]
+}
+
+var  {:layer 0,2} betsStatus   : [Bid]int;
+var  {:layer 0,2} time         : int;
+
+const unique expiryTime   : int;
+const unique P0           : Pid;  // This is the only process that can call settleBet
+
+
+procedure {:atomic}{:layer 2}  placeBet({:linear "Pid"} pid: Pid, {:linear "Bid"} bid: Bid, amount: int)
+modifies betsStatus, time;
+{    
+    assume (pid != P0);
+    assume (time < expiryTime);
+	betsStatus[bid] := amount;
+	time := time + 1;
+}
+procedure {:yields}{:layer 1} {:refines "placeBet"} PlaceBet({:linear "Pid"} pid: Pid, {:linear "Bid"} bid: Bid, amount: int);
+
+
+procedure {:atomic}{:layer 2}  settleBet({:linear "Pid"} pid: Pid) returns (winner:int)
+modifies betsStatus, time;
+{    
+    var bid : Bid;
+    assume (pid == P0);
+    assume (time >= expiryTime);
+	assume (betsStatus[bid] != 0);
+	winner := betsStatus[bid];
+}
+procedure {:yields}{:layer 1} {:refines "settleBet"} SettleBet({:linear "Pid"} pid: Pid) returns (winner:int);
